Connections are now closer than R’s.

low/hooks.ml
@@ -1,0 +1,36 @@
+(** Hooks
+  Contains some impure functions used by the Coq extracted code (mainly input and output). **)
+
+let log = ref false
+
+
+let char_list_to_string str =
+  String.concat "" (List.map (String.make 1) str)
+
+let string_to_char_list str =
+  let rec aux i acc =
+    if i < 0 then acc
+    else aux (i - 1) (str.[i] :: acc) in
+  aux (String.length str - 1) []
+
+
+let generic_print print loc () str =
+  let str = char_list_to_string str in
+  let str =
+    if !log then
+      "Printed message (" ^ loc ^ "): " ^ str
+    else str in
+  print str ;
+  Some ()
+
+let stdout_print = generic_print print_string "stdout"
+let stderr_print = generic_print prerr_string "stderr"
+
+let generic_flush channel loc () =
+  if !log then output_string channel ("Flush (" ^ loc ^ ")") ;
+  flush channel ;
+  Some ()
+
+let stdout_flush = generic_flush stdout "stdout"
+let stderr_flush = generic_flush stderr "stderr"
+
